sms/ssr_sms_1_dsk.v
@@ -49,6 +49,7 @@ Definition sample1 :=
      ipush tn 1;
      ipush tn 2;
      iadd;
+     idrop;
      idrop
   ].
 
@@ -67,6 +68,7 @@ Definition fact :=
               idup;
               ineq
            ];
+     idrop;
      idrop
   ].
 
@@ -97,21 +99,21 @@ Inductive step : relation env :=            (* env -> env -> Prop *)
                            step (us, v2 :: v1 :: vs, iswap :: cs) (us, v1 :: v2 :: vs, cs)
 | steppush_n us n vs cs:   step (us, vs, ipush tn (vn n) :: cs)   (us, (vn n) :: vs, cs)
 | steppush_b us b vs cs:   step (us, vs, ipush tb (vb b) :: cs)   (us, (vb b) :: vs, cs)
-| steploop_tt us vs cs1 cs2 cs : cs1 ++ cs2 = cs ->
+| steploop_tt us vs cs1 cs2 cs : cs1 ++ (iloop cs1 :: cs2) = cs ->
                            step (us, vb true :: vs, iloop cs1 :: cs2) (us, vs, cs)
 | steploop_ff us vs cs1 cs2 :
                            step (us, vb false :: vs, iloop cs1 :: cs2) (us, vs, cs2)
 | stepdip us v vs1 vs2 cs1 cs2 cs : (iup :: cs1) ++ (idown :: cs2) = cs ->
                         step (us, v :: vs1, idip cs1 :: cs2) (vs2, cs)
-| stepadd us v1 v2 v3 vs cs : v1 + v2 = v3 ->
-                        step (us, [::vn v2, vn v1 & vs], iadd :: cs) (us, vn v3 :: vs, cs)
-| stepsub us v1 v2 v3 vs cs : v1 - v2 = v3 ->
-                        step (us, [::vn v2, vn v1 & vs], isub :: cs) (us, vn v3 :: vs, cs)
-| stepmul us v1 v2 v3 vs cs : v1 * v2 = v3 ->
-                        step (us, [::vn v2, vn v1 & vs], imul :: cs) (us, vn v3 :: vs, cs)
+| stepadd us n1 n2 n3 vs cs : n2 + n1 = n3 ->
+                        step (us, [::vn n2, vn n1 & vs], iadd :: cs) (us, vn n3 :: vs, cs)
+| stepsub us n1 n2 n3 vs cs : n2 - n1 = n3 ->
+                        step (us, [::vn n2, vn n1 & vs], isub :: cs) (us, vn n3 :: vs, cs)
+| stepmul us n1 n2 n3 vs cs : n2 * n1 = n3 ->
+                        step (us, [::vn n2, vn n1 & vs], imul :: cs) (us, vn n3 :: vs, cs)
 | stepeq_tt us vs cs :     step (us, vn 0 :: vs, ieq :: cs)     (us, vb true :: vs, cs)
-| stepeq_ff us v vs cs :   step (us, vn v.+1 :: vs, ieq :: cs)  (us, vb false :: vs, cs)
-| stepneq_tt us v vs cs :  step (us, vn v.+1 :: vs, ineq :: cs) (us, vb true :: vs, cs)
+| stepeq_ff us n vs cs :   step (us, vn n.+1 :: vs, ieq :: cs)  (us, vb false :: vs, cs)
+| stepneq_tt us n vs cs :  step (us, vn n.+1 :: vs, ineq :: cs) (us, vb true :: vs, cs)
 | stepneq_ff us vs cs :    step (us, vn 0 :: vs, ineq :: cs)    (us, vb false :: vs, cs)
 | stepup us v vs cs :      step (us, v :: vs, iup :: cs)        (v :: us, vs, cs)
 | stepdown u us vs cs :    step (u :: us, vs, idown :: cs)      (us, u :: vs, cs)
@@ -187,7 +189,7 @@ Proof.
     case: v => [n | b]; first i_none. (* nat か bool で場合分けする。 *)
     left.
     case: b.                      (* true か false で場合分けする。 *)
-    + exists (us, vs, cs1 ++ cs2).
+    + exists (us, vs, cs1 ++ (iloop cs1 :: cs2)).
         by apply: steploop_tt.
     + exists (us, vs, cs2).
         by apply: steploop_ff.
@@ -204,21 +206,21 @@ Proof.
     case: v1; case: v2 => n1 n2; try i_none. (* nat か bool で場合分けする。 *)
     (* nat と nat の組み合わせ以外を try i_none で片付ける。 *)
     left.
-    exists (us, vn (n1 + n2) :: vs, cs).
+    exists (us, vn (n2 + n1) :: vs, cs).
       by apply: stepadd.
   (* sub *)
   - case: vs => [cs | v1 vs cs]; first i_none.
     case: vs => [| v2 vs]; first i_none.
     case: v1; case: v2 => n1 n2; try i_none.
     left.
-    exists (us, vn (n1 - n2) :: vs, cs).
+    exists (us, vn (n2 - n1) :: vs, cs).
       by apply: stepsub.
   (* mul *)
   - case: vs => [cs | v1 vs cs]; first i_none.
     case: vs => [| v2 vs]; first i_none.
     case: v1; case: v2 => n1 n2; try i_none.
     left.
-    exists (us, vn (n1 * n2) :: vs, cs).
+    exists (us, vn (n2 * n1) :: vs, cs).
       by apply: stepmul.
   (* eq *)
   - case: vs => [cs | v vs cs]; first i_none.
@@ -250,5 +252,90 @@ Proof.
     exists (us, [:: u & vs], cs).
       by apply: stepdown.
 Defined.
+
+Print refl_step_closure.
+
+
+Goal ([::], [::], fact) |=>* ([::], [::], [::]).
+Proof.
+  rewrite /fact.
+  apply rsc_step with
+      (y:=([::], [:: vn 1],
+           [:: ipush tn 4; idup; ineq;
+            iloop [:: idup; idip [:: imul]; ipush tn 1; iswap; isub; idup; ineq];
+            idrop; idrop]));
+    first by apply: steppush_n.
+  apply rsc_step with
+      (y:=([::], [:: vn 4; vn 1],
+           [:: idup; ineq;
+            iloop [:: idup; idip [:: imul]; ipush tn 1; iswap; isub; idup; ineq];
+            idrop; idrop]));
+    first by apply: steppush_n.
+  apply rsc_step with
+      (y:=([::], [:: vn 4; vn 4; vn 1],
+           [:: ineq;
+            iloop [:: idup; idip [:: imul]; ipush tn 1; iswap; isub; idup; ineq];
+            idrop; idrop]));
+    first by apply: stepdup.
+  apply rsc_step with
+      (y:=([::], [:: vb true; vn 4; vn 1],
+           [:: iloop [:: idup; idip [:: imul]; ipush tn 1; iswap; isub; idup; ineq];
+            idrop; idrop]));
+    first by apply: stepneq_tt.
+  apply rsc_step with
+      (y:=([::], [:: vn 4; vn 1],
+           [:: idup; idip [:: imul]; ipush tn 1; iswap; isub; idup; ineq;
+            iloop [:: idup; idip [:: imul]; ipush tn 1; iswap; isub; idup; ineq];
+            idrop; idrop]));
+    first by apply: steploop_tt.
+  apply rsc_step with
+      (y:=([::], [:: vn 4; vn 4; vn 1],
+           [:: idip [:: imul]; ipush tn 1; iswap; isub; idup; ineq;
+            iloop [:: idup; idip [:: imul]; ipush tn 1; iswap; isub; idup; ineq];
+            idrop; idrop]));
+    first by apply: stepdup.
+  apply rsc_step with
+      (y:=([::], [:: vn 4; vn 4; vn 1],
+           [:: iup; imul; idown; ipush tn 1; iswap; isub; idup; ineq;
+            iloop [:: idup; idip [:: imul]; ipush tn 1; iswap; isub; idup; ineq];
+            idrop; idrop]));
+    first by apply: stepdip.
+  apply rsc_step with
+      (y:=([:: vn 4], [:: vn 4; vn 1],
+           [:: imul; idown; ipush tn 1; iswap; isub; idup; ineq;
+            iloop [:: idup; idip [:: imul]; ipush tn 1; iswap; isub; idup; ineq];
+            idrop; idrop]));
+    first by apply: stepup.
+  apply rsc_step with
+      (y:=([:: vn 4], [:: vn 4],
+           [:: idown; ipush tn 1; iswap; isub; idup; ineq;
+            iloop [:: idup; idip [:: imul]; ipush tn 1; iswap; isub; idup; ineq];
+            idrop; idrop]));
+    first by apply: stepmul.
+  apply rsc_step with
+      (y:=([::], [:: vn 4; vn 4],
+           [:: ipush tn 1; iswap; isub; idup; ineq;
+            iloop [:: idup; idip [:: imul]; ipush tn 1; iswap; isub; idup; ineq];
+            idrop; idrop]));
+    first by apply: stepdown.
+  apply rsc_step with
+      (y:=([::], [:: vn 1; vn 4; vn 4],
+           [:: iswap; isub; idup; ineq;
+            iloop [:: idup; idip [:: imul]; ipush tn 1; iswap; isub; idup; ineq];
+            idrop; idrop]));
+    first by apply: steppush_n.
+  apply rsc_step with
+      (y:=([::], [:: vn 4; vn 1; vn 4],
+           [:: isub; idup; ineq;
+            iloop [:: idup; idip [:: imul]; ipush tn 1; iswap; isub; idup; ineq];
+            idrop; idrop]));
+    first by apply: stepswap.
+  apply rsc_step with
+      (y:=([::], [:: vn 3; vn 4],
+           [:: idup; ineq;
+            iloop [:: idup; idip [:: imul]; ipush tn 1; iswap; isub; idup; ineq];
+            idrop; idrop]));
+    first by apply: stepsub.
+  Admitted.
 
 (* END *)
